introduced eqtype in universe tutorial examples, Samin does batch from above

doc/tutorial/code/solutions_universes/Ex6c.fst
@@ -1,8 +1,8 @@
 module Ex6c
 
 
-val mem: 'a -> list 'a -> Tot bool
-let rec mem a l = match l with
+val mem: #t:eqtype-> t -> list t -> Tot bool
+let rec mem #t a l = match l with
   | [] -> false
   | hd::tl -> hd=a || mem a tl
 
@@ -14,12 +14,12 @@ let rec append l1 l2 = match l1 with
   | hd :: tl -> hd :: hd :: append tl l2
 
 
-val append_mem:  l1:list 'a
-              -> l2:list 'a
+val append_mem:  #t:eqtype -> l1:list t
+              -> l2:list t
               -> Lemma (requires True)
                        (ensures (forall a. mem a (append l1 l2) = (mem a l1 || mem a l2)))
                        [SMTPat (append l1 l2)]
-let rec append_mem l1 l2 = match l1 with
+let rec append_mem #t l1 l2 = match l1 with
   | [] -> ()
   | hd::tl -> append_mem tl l2
 
@@ -47,15 +47,15 @@ let rec partition f = function
      else l1, hd::l2
 
 
-val partition_lemma: f:('a -> Tot bool)
-                   -> l:list 'a
+val partition_lemma: #t:eqtype -> f:(t -> Tot bool)
+                   -> l:list t
                    -> Lemma (requires True)
                             (ensures ((length (fst (partition f l)) + length (snd (partition f l)) = length l
                                   /\ (forall x. mem x (fst (partition f l)) ==> f x)
                                   /\ (forall x. mem x (snd (partition f l)) ==> not (f x))
                                   /\ (forall x. mem x l = (mem x (fst (partition f l)) || mem x (snd (partition f l)))))))
                             [SMTPat (partition f l)]
-let rec partition_lemma f l = match l with
+let rec partition_lemma #t f l = match l with
     | [] -> ()
     | hd::tl -> partition_lemma f tl
 
